QAux/QAux.thy
@@ -1,6 +1,6 @@
 theory QAux
 imports HOL.Complex  HOL.Orderings  
           Deep_Learning.Tensor_Matricization Separation_Algebra.Separation_Algebra
-          QHLProver.Partial_State  HOL.Finite_Set "HOL-Library.Word"
+          QHLProverSep.Partial_State  HOL.Finite_Set "HOL-Library.Word"
 begin 
 end
